theories/otherversions/nonempty.v
@@ -100,27 +100,16 @@ Proof.
   apply p.
 Qed.
 
-(* The "Unique" monad, that represents a unique thing that exists non-constructively *)
+(* Monad for choice *)
 Definition Classical (A : Type) : Type :=
-  {S : A -> CProp | PClassical (exists a, isTrue (S a))
-                    /\ forall x y, isTrue (S x) /\ isTrue (S y) -> PClassical (x = y)}.
+  {S : A -> CProp | PClassical (exists a, isTrue (S a))}.
 
 Definition Creturn {A : Type} (x : A) : Classical A.
   refine (exist _ (fun y => toCProp (y = x)) _).
-  split.
-  - apply Preturn.
-    exists x.
-    simpl.
-    apply Preturn.
-    reflexivity.
-  - intros.
-    destruct H.
-    simpl in *.
-    apply (Pbind H); clear H; intros H.
-    apply (Pbind H0); clear H0; intros H0.
-    apply Preturn.
-    subst.
-    reflexivity.
+  apply Preturn.
+  exists x.
+  apply Preturn.
+  reflexivity.
 Defined.
 
 (* TODO: Confirm that the output really has to be in PClassical. *)
@@ -140,37 +129,24 @@ Qed.
 Definition Cbind {A B : Type} (pa : Classical A) (f : A -> Classical B) : Classical B.
   refine (exist _ (fun b => toCProp
                               (exists a, isTrue (proj1_sig pa a) /\ isTrue (proj1_sig (f a) b))) _).
-  destruct pa as [Sa [nonempty same]].
+  destruct pa as [Sa nonempty].
+  apply (Pbind nonempty).
+  intros.
   simpl.
-  split.
-  - apply (Pbind nonempty).
-    intros.
-    simpl.
-    destruct H.
-    remember (f x) as fx.
-    destruct fx as [x0 [p sfsdfd]].
-    apply (Pbind p).
-    intros.
-    apply Preturn.
-    destruct H0.
-    exists x1.
-    apply Preturn.
-    exists x.
-    split; auto.
-    rewrite <- Heqfx.
-    simpl.
-    assumption.
-  - intros x y [allx ally].
-    apply (Pbind allx); clear allx; intros [ax [Saax fax]].
-    apply (Pbind ally); clear ally; intros [ay [Saay fay]].
-    specialize (same _ _ (conj Saax Saay)).
-    apply (Pbind same); clear same; intro same.
-    subst.
-    apply (Pbind (proj2 (proj2_sig (f ay)) _ _ (conj fax fay))).
-    intros.
-    subst.
-    apply Preturn.
-    reflexivity.
+  destruct H.
+  remember (f x) as fx.
+  destruct fx.
+  apply (Pbind p).
+  intros.
+  apply Preturn.
+  destruct H0.
+  exists x1.
+  apply Preturn.
+  exists x.
+  split; auto.
+  rewrite <- Heqfx.
+  simpl.
+  assumption.
 Defined.
 
 (* one of the monad laws *)
@@ -203,6 +179,51 @@ Proof.
     + assumption.
 Qed.
 
+(* TODO: Should P output a CProp? *)
+Definition choose (T : Type) (P : T -> Prop) (H : PClassical (exists t, P t)): Classical T.
+  refine (exist _ (fun t => toCProp (P t)) _).
+  apply (Pbind H); clear H; intros H.
+  destruct H as [t Pt].
+  apply Preturn.
+  exists t.
+  simpl.
+  apply Preturn.
+  assumption.
+Defined.
+
+Theorem choice_spec (T : Type) (P : T -> Prop) (H : PClassical (exists t, P t))
+  : Cbind (choose T P H) (fun t => Creturn (P t)) = Creturn True.
+Proof.
+  apply sigEq2.
+  simpl.
+  extensionality X.
+  apply CProp_Ext.
+  - intros.
+    simpl in *.
+    apply (Pbind H0); clear H0; intros H0.
+    destruct H0.
+    destruct H0.
+    apply (Pbind H1); clear H1; intros H1.
+    apply (Pbind H0); clear H0; intros H0.
+    subst.
+    apply Preturn.
+    apply propositional_extensionality; split; auto.
+  - intros.
+    subst.
+    simpl in *.
+    apply (Pbind H); clear H; intros H.
+    destruct H.
+    apply (Pbind H0); clear H0; intros H0.
+    apply Preturn.
+    exists x.
+    subst.
+    split.
+    + apply Preturn.
+      assumption.
+    + apply Preturn.
+      apply propositional_extensionality; split; auto.
+Qed.
+
 Theorem monadlaw2 (T : Type) (t : Classical T) : Cbind t Creturn = t.
 Proof.
   apply sigEq2.
@@ -227,81 +248,88 @@ Proof.
     reflexivity.
 Qed.
 
-(* Can I get this for this version? *)
-Theorem ClassicalInd T (t : Classical T)
-  : PClassical (exists x, Creturn x = t /\ (isTrue (proj1_sig t x))).
+Theorem writeInTermsOfBind (T : Type) (t1 t2 : Classical T)
+        (H : Cbind t1 Creturn = Cbind t2 Creturn)
+  : t1 = t2.
 Proof.
-  destruct t as [St [nonempty same]].
-  apply (Pbind nonempty); intros [a ta].
-  apply Preturn.
-  exists a.
-  split.
-  - 
-    apply sigEq2.
-    simpl.
-    extensionality t.
-    apply CProp_Ext.
-    + simpl.
-      intros.
-      apply unwrap.
-      apply (Pbind H); clear H; intros H.
-      subst.
-      apply Preturn.
-      assumption.
-    + intros.
-      simpl.
-      specialize (same _ _ (conj ta H)).
-      apply (Pbind same); clear same; intros same.
-      subst.
-      apply Preturn.
-      reflexivity.
-  - simpl.
-    assumption.
-Qed.
-
-(* unique choice *)
-Definition choose (T : Type) (P : T -> Prop)
-           (nonempty : PClassical (exists t, P t))
-           (unique : forall x y, P x /\ P y -> PClassical (x = y))
-  : Classical T.
-  refine (exist _ (fun t => toCProp (P t)) _).
-  split.
-  - simpl.
-    apply (Pbind nonempty); clear nonempty; intros [t Pt].
-    apply Preturn.
-    exists t.
-    apply Preturn.
-    assumption.
-  - intros x y [Px Py].
-    simpl in *.
-    apply (Pbind Px); clear Px; intros Px.
-    apply (Pbind Py); clear Py; intros Py.
-    specialize (unique _ _ (conj Px Py)).
-    assumption.
-Defined.
-
-Theorem choiceInd : forall (T : Type) (P : T -> Prop) (Q : Classical T -> Prop)
-                            nonempty unique,
-    (forall t, P t -> PClassical (Q (Creturn t)))
-    -> PClassical (Q (@choose T P nonempty unique)).
-Proof.
-  intros.
-  apply (Pbind (ClassicalInd _ (choose T P nonempty unique))).
-  simpl.
-  intros [St [eq PSt]].
-  rewrite <- eq.
-  clear eq.
-  apply (Pbind nonempty); clear nonempty; intros [t Pt].
-  specialize (H _ Pt).
-  apply (Pbind H); clear H; intros H.
-  pbind PSt.
-  specialize (unique _ _ (conj Pt PSt)).
-  pbind unique.
-  subst.
-  apply Preturn.
+  repeat rewrite monadlaw2 in H.
   assumption.
 Qed.
 
+Theorem choiceInd (A B : Type) (P : A -> Prop)
+        {H : PClassical (exists a, P a)}
+        {rest : A -> Classical B}
+        {v : Classical B}
+        (premise : forall x, P x -> rest x = v)
+  : Cbind (choose _ P H) rest = v.
+Proof.
+  apply sigEq2.
+  simpl.
+  extensionality b.
+  apply CProp_Ext.
+  - intros.
+    apply unwrap.
+    simpl in *.
+    apply (Pbind H0); clear H0; intros H0.
+    destruct H0.
+    destruct H0.
+    apply (Pbind H0); clear H0; intros H0.
+    specialize (premise x H0).
+    subst.
+    apply Preturn.
+    assumption.
+  - intros.
+    simpl in *.
+    apply (Pbind H); clear H; intros H.
+    apply Preturn.
+    destruct H.
+    exists x.
+    split.
+    + apply Preturn.
+      assumption.
+    + specialize (premise x H).
+      subst.
+      assumption.
+Qed.
+(*
+(* Is it possible to prove something like this? *)
+Theorem choiceInd2 : forall (T : Type) (P : T -> Prop) (Q : T -> CProp) x,
+    (forall t, P t -> isTrue (Q t)) -> isTrue (Cbind (@choose T P x) Q).
+Abort.
+(* Maybe something like this: *)
+Theorem choice_spec (T : Type) (P : T -> CProp) (H : PClassical (exists t, P t))
+  : isTrue (Cbind (choose T P H) P).
+ *)
+
+Theorem choiceInd2 : forall (T : Type) (P : T -> Prop) (Q : Classical T -> Prop)
+                            nonempty
+                            (unique : forall x y, P x -> P y -> PClassical (x = y)),
+    (forall t, P t -> PClassical (Q (Creturn t)))
+    -> PClassical (Q (@choose T P nonempty)).
+Proof.
+  intros.
+  apply (Pbind nonempty). intros [t Pt].
+  specialize (H t Pt).
+
+  assert (choose T P nonempty = Creturn t). {
+    apply sigEq2.
+    simpl.
+    extensionality t'.
+    apply CProp_Ext.
+    simpl.
+    - intros.
+      pbind H0.
+      apply unique; assumption.
+    - simpl.
+      intros.
+      pbind H0.
+      subst.
+      apply Preturn.
+      assumption.
+  }
+  rewrite H0.
+  assumption.
+Qed.
 
 Inductive whileR {A B : Type} (step : A -> A + B) : A -> B -> Prop :=
 | while_base : forall a b, step a = inr b -> whileR step a b
@@ -339,71 +367,67 @@ Definition while {A B : Type} (a : A) (step : A -> A + B) : Partial B.
   refine (choose _ (fun ob => match ob with
                               | None => ~ exists b, whileR step a b
                               | Some b => whileR step a b
-                              end) _ _).
-  - apply (Pbind (Plem (exists b, whileR step a b))); intros.
-    destruct H.
-    + destruct H.
-      apply Preturn.
-      exists (Some x).
-      assumption.
-    + apply Preturn.
-      exists None.
-      assumption.
-  - intros x y [whilex whiley].
-    destruct x, y.
-    + rewrite (whileRFunction _ _ _ _ _ _ whilex whiley).
-      apply Preturn.
-      reflexivity.
-    + destruct whiley.
-      exists b.
-      assumption.
-    + destruct whilex.
-      exists b.
-      assumption.
-    + apply Preturn.
-      reflexivity.
+                              end) _).
+  apply (Pbind (Plem (exists b, whileR step a b))); intros.
+  destruct H.
+  - destruct H.
+    apply Preturn.
+    exists (Some x).
+    assumption.
+  - apply Preturn.
+    exists None.
+    assumption.
 Defined.
 
 Theorem whileBase (A B : Type) step (a : A) (b : B)
         (H : step a = inr b)
-  : PClassical (while a step = Creturn (Some b)).
+  : while a step = Creturn (Some b).
 Proof.
-  apply (choiceInd (option B) _ (fun c => c = Creturn (Some b))).
+  apply writeInTermsOfBind.
+  rewrite bindDef.
+  unfold while.
+  rewrite @choiceInd with (v := Creturn (Some b)).
+  reflexivity.
   intros.
-  apply while_base in H.
-  destruct t.
-  - rewrite (whileRFunction _ _ _ _ _ _ H H0).
-    apply Preturn.
+  apply f_equal.
+  destruct x.
+  - rewrite (whileRFunction _ _ _ _ _ _ (while_base _ _ _ H) H0).
     reflexivity.
-  - destruct H0.
+  - apply while_base in H.
+    exfalso.
+    apply H0.
     exists b.
     assumption.
 Qed.
 
 Theorem whileStep (A B : Type) step (a a' : A)
         (H : step a = inl a')
-  : PClassical (@while A B a step = while a' step).
+  : @while A B a step = while a' step.
 Proof.
-  apply choiceInd.
+  apply writeInTermsOfBind.
+  Check choiceInd.
+  unfold while.
+  erewrite choiceInd; try reflexivity.
+  symmetry.
+  erewrite choiceInd; try reflexivity.
   intros.
-  apply (choiceInd _ _ (fun c => c = Creturn t)).
-  intros.
-  destruct t, t0.
-  - rewrite (whileRFunction _ _ _ _ _ _ (while_step _ _ _ _ H H0) H1).
-    apply Preturn.
+  symmetry.
+  apply f_equal.
+
+  destruct x, x0.
+  - rewrite (whileRFunction _ _ _ _ _ _ (while_step _ _ _ _ H H1) H0).
     reflexivity.
   - destruct H1.
-    exists b.
-    apply (while_step _ _ _ _ H H0).
+    inversion H0.
+    + rewrite H in H1.
+      inversion H1.
+    + rewrite H in H1.
+      inversion H1.
+      subst.
+      exists b.
+      assumption.
   - destruct H0.
     exists b.
-    destruct H1.
-    + rewrite H in H0.
-      inversion H0.
-    + rewrite H in H0.
-      inversion H0.
-      subst.
-      assumption.
-  - apply Preturn.
-    reflexivity.
+    apply while_step with (a' := a'); assumption.
+  - reflexivity.
 Qed.
